chore: switch arg order for updateBins

Earley/Recognizer.lean
@@ -288,8 +288,8 @@ public def updateBin (xs : List (BinItem T N)) : List (BinItem T N) → List (Bi
 Replace `bins` at index `k` with `newBin` and return the updated bins.
 -/
 @[grind]
-public def updateBins {n : Nat} (bins : EarleyBins T N n) (k : Nat) (newBin : List (BinItem T N))
-    (hk : k < n) : EarleyBins T N n :=
+public def updateBins {n : Nat} (bins : EarleyBins T N n) (k : Nat) (hk : k < n)
+    (newBin : List (BinItem T N)) : EarleyBins T N n :=
   let newBin := updateBin bins[k] newBin
   bins.set k newBin hk
 
@@ -389,7 +389,7 @@ lemma length_le_lengthUpdateBin (xs ys : List (BinItem T N)) :
 omit [LawfulBEq (EarleyItem T N)] in
 lemma lengthNth_le_lengthUpdateBinNth {n : Nat} (bins : EarleyBins T N n) (ys : List (BinItem T N))
     (i k : Nat) (hi : i < n) (hk : k < n) :
-    bins[i].length ≤ (updateBins bins k ys hk)[i].length := by
+    bins[i].length ≤ (updateBins bins k hk ys)[i].length := by
   induction ys generalizing bins with
   | nil => grind
   | cons x xs ih => grind [length_le_lengthUpdateBinAux, length_le_lengthUpdateBin]
@@ -584,18 +584,18 @@ lemma wfBins_of_updateBin (G : ContextFreeGrammarList T N) (w : List T) {k : Nat
     (hwfy : ∀ y ∈ ys, isWellFormed G.rules (mapT w) y.item ∧ y.item.endIdx = k)
     (hwfPy : isWellFormedBinPointers w bins ys k)
     (hwfSy : ∀ y ∈ ys, isSoundPointer y.pointer k bins[k].length) :
-    isWellFormedBins G w (updateBins bins k ys hk)  := by
+    isWellFormedBins G w (updateBins bins k hk ys)  := by
   intro i hi
   if heq : i = k then
     refine ⟨by grind [wfBinItems_of_updateBin], ?_, ?_⟩
     · have ⟨h1,h2,h3⟩ := hwf k (by lia)
       simp only [heq]
-      have hwfb : isWellFormedBinPointers w bins (updateBins bins k ys hk)[k] k := by
+      have hwfb : isWellFormedBinPointers w bins (updateBins bins k hk ys)[k] k := by
         have := wfBinPointers_of_updateBin w bins bins[k] h2 ys (by grind)
         grind
       have : ∀ (i : ℕ) (hi : i ≤ w.length), bins[i].length
-          ≤ (updateBins bins k ys hk)[i].length := by grind [lengthNth_le_lengthUpdateBinNth]
-      have := wfBinPointers_of_updatedBins w bins (updateBins bins k ys hk) hk this hwfb
+          ≤ (updateBins bins k hk ys)[i].length := by grind [lengthNth_le_lengthUpdateBinNth]
+      have := wfBinPointers_of_updatedBins w bins (updateBins bins k hk ys) hk this hwfb
       grind
     · intro j hj
       have := soundPointers_of_updateBin w k bins (by grind) ys
@@ -604,9 +604,9 @@ lemma wfBins_of_updateBin (G : ContextFreeGrammarList T N) (w : List T) {k : Nat
     refine ⟨by grind, ?_⟩
     have ⟨h1,h2⟩ := hwf k (by lia)
     have hi : i < w.length + 1 := by lia
-    have : ∀ (i : ℕ) (hi : i ≤ w.length), bins[i].length ≤ (updateBins bins k ys hk)[i].length := by
+    have : ∀ (i : ℕ) (hi : i ≤ w.length), bins[i].length ≤ (updateBins bins k hk ys)[i].length := by
       grind [lengthNth_le_lengthUpdateBinNth]
-    have := wfBinPointers_of_updatedBins w bins (updateBins bins k ys hk) hi this
+    have := wfBinPointers_of_updatedBins w bins (updateBins bins k hk ys) hi this
     grind
 
 omit [BEq T] in
@@ -640,7 +640,7 @@ lemma wfBins_of_scanList {G : ContextFreeGrammarList T N} {w : List T} {j k : Na
     {bins : EarleyBins T N (w.length + 1)} (hbins : isWellFormedBins G w bins)
     (x : EarleyItem T N) (hk : k < w.length) (hj : ¬ (j ≥ bins[k].length))
     (hx : x = (bins[k][j]).item) (hnext : nextSymbol x = some (Symbol.terminal a)) :
-    isWellFormedBins G w (updateBins bins (k+1) (scanList w x a k hk j) (by lia)) := by
+    isWellFormedBins G w (updateBins bins (k+1) (by lia) (scanList w x a k hk j)) := by
   apply wfBins_of_updateBin G w bins hbins (scanList w x a k hk j) (by lia)
   · exact wfItems_of_scanList j k hbins x hk (by grind) hnext
   · grind [wfPointers_of_scanList]
@@ -668,7 +668,7 @@ lemma soundPointers_of_predictList (G : ContextFreeGrammarList T N) {w : List T}
 lemma wfBins_of_predictList {G : ContextFreeGrammarList T N} {w : List T} {A : N} {k : Nat}
     {bins : EarleyBins T N (w.length + 1)} (hbins : isWellFormedBins G w bins)
     (hk : k < w.length + 1) :
-    isWellFormedBins G w (updateBins bins k (predictList G A k) (by lia)) := by
+    isWellFormedBins G w (updateBins bins k hk (predictList G A k)) := by
   apply wfBins_of_updateBin G w bins hbins (predictList G A k) hk
   · grind [wfItems_of_predictList]
   · grind [wfPointers_of_predictList]
@@ -745,10 +745,10 @@ lemma wfBins_of_completeList {G : ContextFreeGrammarList T N} {w : List T} {j k 
     {bins : EarleyBins T N (w.length + 1)} (hbins : isWellFormedBins G w bins)
     (y : EarleyItem T N) (hk : k < bins.size) (hj : ¬ (j ≥ bins[k].length))
     (hy : y = bins[k][j].item) : isWellFormedBins G w
-    (updateBins bins k (completeList y bins (by grind) j) (by lia)) := by
+    (updateBins bins k hk (completeList y bins (by grind) j)) := by
   apply wfBins_of_updateBin G w bins hbins (completeList y bins (by grind) j) hk
   · grind [wfItems_of_completeList j k hbins y]
-  · grind [wfPointers_of_completeList j k hbins y hk (by grind) (by omega)]
+  · grind [wfPointers_of_completeList j k hbins y hk (by grind) (by lia)]
   · grind [soundPointers_of_completeList G j k bins hbins y hk]
 
 lemma wfBins_of_earleyBinList {G : ContextFreeGrammarList T N} {w : List T} (j k : Nat)
@@ -760,16 +760,16 @@ lemma wfBins_of_earleyBinList {G : ContextFreeGrammarList T N} {w : List T} (j k
       | some s => match s with
         | Symbol.nonterminal A =>
           let newItems := predictList G A k
-          updateBins bins k newItems (by omega)
+          updateBins bins k hk newItems
         | Symbol.terminal a =>
           if hk : k ≥ w.length then
             bins
           else
-            let newItem := scanList w x.item a k (by omega) j
-            updateBins bins (k + 1) newItem (by omega)
+            let newItem := scanList w x.item a k (by lia) j
+            updateBins bins (k + 1) (by lia) newItem
       | none =>
         let newItems := completeList x.item bins (by grind) j
-        updateBins bins k newItems (by omega)) :
+        updateBins bins k hk newItems) :
     isWellFormedBins G w bins' := by
   simp only [h, ge_iff_le]
   match hnext : nextSymbol bins[k][j].item with
@@ -827,7 +827,7 @@ lemma decreasingAux {G : ContextFreeGrammarList T N} {w : List T}
 Computes the k-th bin starting from index j and returns the updated bins.
 -/
 public def earleyBinList (G : ContextFreeGrammarList T N) (w : List T) (k : Nat)
-    (bins : EarleyBins T N (w.length + 1)) (h : k < bins.size) (j : Nat)
+    (bins : EarleyBins T N (w.length + 1)) (hk : k < bins.size) (j : Nat)
     (hbins : isWellFormedBins G w bins) : WfEarleyBins G w :=
   -- Return the bins if we are the end of the list of the current bin
   if hj : j ≥ bins[k].length then
@@ -839,21 +839,21 @@ public def earleyBinList (G : ContextFreeGrammarList T N) (w : List T) (k : Nat)
       | Symbol.nonterminal A =>
         -- Add all potential .predict operations on the current item to the current bin
         let newItems := predictList G A k
-        updateBins bins k newItems (by omega)
+        updateBins bins k hk newItems
       | Symbol.terminal a =>
         -- If we are the final bin then don't try to progress via consuming another terminal
         if hk : k ≥ w.length then
           bins
         else
           -- Add a potential .scan operations on the current item to the next bin
-          let newItem := scanList w x.item a k (by omega) j
-          updateBins bins (k+1) newItem (by omega)
+          let newItem := scanList w x.item a k (by lia) j
+          updateBins bins (k+1) (by lia) newItem
     | none =>
       -- Add all potential .complete operations on the current item to the current bin
       let newItems := completeList x.item bins (by grind) j
-      updateBins bins k newItems (by omega)
+      updateBins bins k hk newItems
     have : isWellFormedBins G w bins' := by grind [wfBins_of_earleyBinList]
-    earleyBinList G w k bins' (by omega) (j+1) this
+    earleyBinList G w k bins' (by lia) (j+1) this
 termination_by { x | isWellFormed G.rules (mapT w) x }.ncard + 1 - j
 decreasing_by exact decreasingAux hbins j k (by lia) (by lia)
 
